Test_PRHL.thy
@@ -4,93 +4,62 @@ begin
 
 record memory = mem_x :: int   mem_y :: "real"   mem_z :: nat
 
-definition "x_raw (m::memory) = (mem_x m, m\<lparr>mem_x := 0\<rparr>)"
-lemma valid_x_raw: "valid_var (x_raw, UNIV)"
-  unfolding valid_var_def x_raw_def case_prod_conv
-  apply (rule exI[of _ "{m\<lparr>mem_x := 0\<rparr> | m. True}"])
-  apply (rule bij_betw_byWitness[where f'="\<lambda>(v,m). m\<lparr>mem_x := v\<rparr>"])
-  by auto
+
+definition "x_raw = (mem_x, \<lambda>a m. m\<lparr>mem_x := a\<rparr>)"
+
+lemma valid_x_raw: "valid_raw_var (UNIV, x_raw)"
+  unfolding x_raw_def apply (rule valid_raw_varI) by auto
 
 lift_definition x :: "(memory,int) var" is x_raw
-  by (rule valid_x_raw)
+  using valid_x_raw by auto
 
-lemma [simp]: "has_variables TYPE(memory) TYPE(int)"
-  using valid_x_raw by auto  
+lemma [simp]: "valid_var x"
+  apply transfer using valid_x_raw by auto  
 
 lemma [simp]: "eval_var x m = mem_x m"
   apply transfer using valid_x_raw unfolding x_raw_def by auto
 
-lemma [simp]: "inj x_raw"
-  using valid_x_raw
-  by (metis (no_types, lifting) Pair_inject iffs injI surjective update_convs(1) x_raw_def)
-
 lemma [simp]: "update_var x a m = m\<lparr>mem_x := a\<rparr>"
-  apply transfer apply (simp add: valid_x_raw)
-  apply (rule inv_f_eq)
-   apply simp
-  unfolding x_raw_def by simp
+  apply transfer unfolding x_raw_def by simp
 
 
+definition "y_raw = (mem_y, \<lambda>a m. m\<lparr>mem_y := a\<rparr>)"
 
-
-
-
-
-
-definition "y_raw (m::memory) = (mem_y m, m\<lparr>mem_y := undefined\<rparr>)"
-lemma valid_y_raw: "valid_var (y_raw, UNIV)"
-  unfolding valid_var_def y_raw_def case_prod_conv
-  apply (rule exI[of _ "{m\<lparr>mem_y := undefined\<rparr> | m. True}"])
-  apply (rule bij_betw_byWitness[where f'="\<lambda>(v,m). m\<lparr>mem_y := v\<rparr>"])
-  by auto
+lemma valid_y_raw: "valid_raw_var (UNIV, y_raw)"
+  unfolding y_raw_def apply (rule valid_raw_varI) by auto
 
 lift_definition y :: "(memory,real) var" is y_raw
-  by (rule valid_y_raw)
+  using valid_y_raw by auto
 
-lemma [simp]: "has_variables TYPE(memory) TYPE(real)"
-  using valid_y_raw by auto  
+lemma [simp]: "valid_var y"
+  apply transfer using valid_y_raw by auto  
 
 lemma [simp]: "eval_var y m = mem_y m"
   apply transfer using valid_y_raw unfolding y_raw_def by auto
 
-lemma [simp]: "inj y_raw"
-  using valid_y_raw
-  by (metis (no_types, lifting) Pair_inject iffs injI surjective update_convs(2) y_raw_def)
-
 lemma [simp]: "update_var y a m = m\<lparr>mem_y := a\<rparr>"
-  apply transfer apply (simp add: valid_y_raw)
-  apply (rule inv_f_eq)
-   apply simp
-  unfolding y_raw_def by simp
+  apply transfer unfolding y_raw_def by simp
 
 
+definition "z_raw = (mem_z, \<lambda>a m. m\<lparr>mem_z := a\<rparr>)"
 
-
-definition "z_raw (m::memory) = (mem_z m, m\<lparr>mem_z := 0\<rparr>)"
-lemma valid_z_raw: "valid_var (z_raw, UNIV)"
-  unfolding valid_var_def z_raw_def case_prod_conv
-  apply (rule exI[of _ "{m\<lparr>mem_z := 0\<rparr> | m. True}"])
-  apply (rule bij_betw_byWitness[where f'="\<lambda>(v,m). m\<lparr>mem_z := v\<rparr>"])
-  by auto
+lemma valid_z_raw: "valid_raw_var (UNIV, z_raw)"
+  unfolding z_raw_def apply (rule valid_raw_varI) by auto
 
 lift_definition z :: "(memory,nat) var" is z_raw
-  by (rule valid_z_raw)
+  using valid_z_raw by auto
 
-lemma [simp]: "has_variables TYPE(memory) TYPE(nat)"
-  using valid_z_raw by auto  
+lemma [simp]: "valid_var z"
+  apply transfer using valid_z_raw by auto  
 
 lemma [simp]: "eval_var z m = mem_z m"
   apply transfer using valid_z_raw unfolding z_raw_def by auto
 
-lemma [simp]: "inj z_raw"
-  using valid_z_raw unfolding valid_var_def case_prod_conv
-  using bij_betw_imp_inj_on by blast 
-
 lemma [simp]: "update_var z a m = m\<lparr>mem_z := a\<rparr>"
-  apply transfer apply (simp add: valid_z_raw)
-  apply (rule inv_f_eq)
-   apply simp
-  unfolding z_raw_def by simp
+  apply transfer unfolding z_raw_def by simp
+
+
+
 
 
 lemma [simp, independence]:
@@ -99,11 +68,13 @@ lemma [simp, independence]:
   "independent_vars y z" "independent_vars z y"
   unfolding independent_vars_def by simp_all
 
+
 lemma [simp]:
   "independent_of mem_x y" "independent_of mem_y x"
   "independent_of mem_x z" "independent_of mem_z x"
   "independent_of mem_y z" "independent_of mem_z y"
   unfolding independent_of_def by simp_all
+
 
 Hoare config (prhl) memory = memory
 
