All.thy
@@ -1,5 +1,5 @@
 theory All
-  imports Test_Reorder_Hoare Test_Tmp_Hoare Demo_Hoare Test
+  imports Test_Reorder_Hoare Test_PRHL Test
 begin
 
 end
