isabelle.sh
@@ -1,1 +1,1 @@
-/opt/Isabelle2020/bin/isabelle jedit -l Lots-Of-Stuff Test_Tmp_Hoare.thy &
+/opt/Isabelle2020/bin/isabelle jedit -l Lots-Of-Stuff Test_PRHL.thy &
